session.v
@@ -1,0 +1,560 @@
+From stdpp Require Import base gmap.
+From mathcomp Require Import ssreflect.
+From iris.algebra Require Import agree auth csum gset gmap excl namespace_map frac.
+From iris.base_logic.lib Require Import auth.
+From iris.heap_lang Require Import notation proofmode.
+From crypto Require Import lib term crypto primitives tactics.
+
+Set Implicit Arguments.
+Unset Strict Implicit.
+Unset Printing Implicit Defensive.
+
+Section Session.
+
+Context `{!cryptoG Σ, !heapG Σ}.
+Notation iProp  := (iProp Σ).
+Notation iPropI := (iPropI Σ).
+
+Inductive role := Init | Resp.
+
+Canonical roleO := leibnizO role.
+
+Implicit Types rl : role.
+
+Global Instance role_inhabited : Inhabited role := populate Init.
+
+Lemma role_equivI rl1 rl2 :
+  rl1 ≡ rl2 ⊣⊢@{iPropI}
+  match rl1, rl2 with
+  | Init, Init | Resp, Resp => True
+  | _, _ => False
+  end.
+Proof.
+by case: rl1 rl2=> [] []; iSplit=> //.
+Qed.
+
+Definition bool_of_role rl :=
+  if rl is Init then true else false.
+
+Definition role_of_bool (b : bool) : role :=
+  if b then Init else Resp.
+
+Lemma bool_of_roleK : Cancel (=) role_of_bool bool_of_role.
+Proof. by case. Qed.
+
+Global Instance role_eq_dec : EqDecision role.
+Proof.
+refine (λ rl1 rl2,
+          match rl1, rl2 with
+          | Init, Init => left _
+          | Resp, Resp => left _
+          | _, _ => right _
+          end); abstract intuition congruence.
+Defined.
+
+Global Instance role_countable : Countable role.
+Proof. apply (inj_countable' _ _ bool_of_roleK). Qed.
+
+Definition swap_role rl :=
+  if rl is Init then Resp else Init.
+
+Inductive session_data := SessionData {
+  srole : role;
+  sinit : term;
+  sresp : term;
+  sdata : option term;
+}.
+
+Canonical session_dataO := leibnizO session_data.
+
+Global Instance session_data_inhabited : Inhabited session_data :=
+  populate (SessionData inhabitant inhabitant inhabitant inhabitant).
+
+Definition sroleo s := swap_role s.(srole).
+
+Definition sowner s :=
+  if s.(srole) is Init then s.(sinit) else s.(sresp).
+
+Definition sother s :=
+  if s.(srole) is Init then s.(sresp) else s.(sinit).
+
+Definition session_data' : Type :=
+  agree role * agree term * agree term * agree (option term).
+
+Definition session_data'R : cmraT :=
+  prodR (prodR (prodR (agreeR roleO) (agreeR termO)) (agreeR termO))
+        (optionR (agreeR termO)).
+
+Implicit Types t : term.
+Implicit Types SM : gmap term session_data.
+Implicit Types s : session_data.
+Implicit Types lvl : level.
+
+Definition session_mapUR :=
+  gmapUR term (authR (optionUR session_data'R)).
+
+Class sessionG := {
+  session_inG  :> inG Σ (authR session_mapUR);
+  session_name :  gname;
+  key_inv      :  role → term → iProp;
+  key_inv_persistent :> ∀ rl t, Persistent (key_inv rl t);
+  sessionN     :  namespace;
+}.
+
+Context `{!sessionG}.
+
+Global Instance sessionG_authG : authG _ _ :=
+  AuthG Σ session_mapUR session_inG _.
+
+Definition to_session_data' s : session_data'R :=
+  (to_agree s.(srole), to_agree s.(sinit),
+   to_agree s.(sresp), to_agree <$> s.(sdata)).
+
+Global Instance to_session_data'_inj : Inj (=) (≡) to_session_data'.
+Proof.
+case=> [??? ot1] [??? ot2]; do 3![case]=> /=.
+do 3![move=> /to_agree_inj ->].
+case: ot2=> [t2|] /=; last first.
+  by move=> /equiv_None; case: ot1.
+case/fmap_Some_equiv=> t1 [-> /to_agree_inj e].
+by apply leibniz_equiv in e; congruence.
+Qed.
+
+Lemma to_session_data'_valid s : ✓ to_session_data' s.
+Proof.
+rewrite /to_session_data'; repeat split=> //=.
+by case: (sdata s).
+Qed.
+
+Lemma to_session_data'_validN n s : ✓{n} to_session_data' s.
+Proof.
+rewrite /to_session_data'; repeat split=> //=.
+by case: (sdata s).
+Qed.
+
+Lemma to_session_data'_included s1 s2 :
+  to_session_data' s1 ≼ to_session_data' s2 ↔
+  s1.(srole) = s2.(srole) ∧
+  s1.(sinit) = s2.(sinit) ∧
+  s1.(sresp) = s2.(sresp) ∧
+  match s1.(sdata) with
+  | Some _ => s1.(sdata) = s2.(sdata)
+  | _ => True
+  end.
+Proof.
+rewrite !pair_included; split.
+- do 3![case]=> /=.
+  rewrite !to_agree_included => -> -> -> edata.
+  repeat split; case: (sdata s1) edata=> [t1|] //=.
+  rewrite option_included; case=> //.
+  destruct 1 as (t1' & s2' & e1 & e2 & e3).
+  case: (sdata s2) e1 e2 e3=> [t2|] //= [<-] [<-].
+  by rewrite to_agree_included; case=> [/to_agree_inj ->|->].
+- do 3![case=> ->]; move=> edata; intuition.
+  rewrite option_included.
+  case: (sdata s1) edata=> [t1|] /=; last by left.
+  by move=> <-; right; exists (to_agree t1), (to_agree t1); eauto.
+Qed.
+
+Lemma to_session_data'_included_eq s1 s2 :
+  to_session_data' s1 ≼ to_session_data' s2 →
+  is_Some s1.(sdata) →
+  s1 = s2.
+Proof.
+move=> eincl [t e].
+case: s1 s2 e eincl => [????] [????] /= ->.
+rewrite to_session_data'_included /=.
+by case=> <- [<- [<- <-]].
+Qed.
+
+Definition session_data_auth s := ● (Some (to_session_data' s)).
+Definition session_data_frag s := ◯ (Some (to_session_data' s)).
+Definition session_data_auth_frag s :=
+  session_data_auth s ⋅ session_data_frag s.
+
+Lemma session_data_auth_included s1 s2 :
+  session_data_auth s1 ≼ session_data_auth_frag s2 ↔ s1 = s2.
+Proof.
+split; last by move=> ->; exists (session_data_frag s2).
+rewrite auth_included /= Some_included.
+destruct 1 as [[[_ e]|e] _].
+- rewrite /= in e.
+  apply to_agree_inj in e.
+  apply Some_equiv_inj in e.
+  by apply to_session_data'_inj in e.
+- move: e; rewrite pair_included; case=> _.
+  rewrite to_agree_included=> e.
+  by apply Some_equiv_inj, to_session_data'_inj in e.
+Qed.
+
+Lemma session_data_frag_included s1 s2 :
+  session_data_frag s1 ≼ session_data_auth_frag s2 ↔
+  to_session_data' s1 ≼ to_session_data' s2.
+Proof.
+split.
+- rewrite auth_included.
+  case=> _ /=; rewrite ucmra_unit_left_id.
+  by rewrite Some_included; case=> [->|].
+- move=> e; transitivity (session_data_frag s2).
+    by rewrite auth_included /= Some_included; eauto.
+  by exists (session_data_auth s2); rewrite cmra_comm.
+Qed.
+
+Lemma session_data_auth_valid s : ✓ session_data_auth s.
+Proof.
+rewrite auth_valid_eq /=; split=> // n.
+exists (Some (to_session_data' s)); split=> //.
+split.
+- by exists (Some (to_session_data' s)); rewrite ucmra_unit_left_id.
+- apply Some_validN, to_session_data'_validN.
+Qed.
+
+Lemma session_data_frag_valid s : ✓ session_data_frag s.
+Proof. by apply auth_frag_valid, to_session_data'_valid. Qed.
+
+Lemma session_data_valid s1 s2 :
+  ✓ (session_data_auth s1 ⋅ session_data_frag s2) ↔
+  to_session_data' s2 ≼ to_session_data' s1.
+Proof.
+rewrite auth_both_valid Some_included; split.
+- by case=> [[->|?] _].
+- move=> e; intuition eauto.
+  rewrite Some_valid; exact: to_session_data'_valid.
+Qed.
+
+Lemma session_data_auth_frag_valid s : ✓ session_data_auth_frag s.
+Proof. exact/session_data_valid. Qed.
+
+Definition to_session_map SM : gmap term _ :=
+  session_data_auth_frag <$> SM.
+
+Definition session_auth t s : iProp :=
+  auth_own session_name {[t := session_data_auth s]}.
+
+Definition session_frag t s : iProp :=
+  auth_own session_name {[t := session_data_frag s]}.
+
+Global Instance session_frag_persistent t s :
+  Persistent (session_frag t s).
+Proof. apply _. Qed.
+
+Lemma session_agree t s1 s2 :
+  session_auth t s1 -∗
+  session_frag t s2 -∗
+  ⌜to_session_data' s2 ≼ to_session_data' s1⌝.
+Proof.
+iIntros "Hown1 Hown2".
+iPoseProof (own_valid_2 with "Hown1 Hown2") as "%Hvalid".
+iPureIntro; apply/session_data_valid.
+by rewrite auth_valid_discrete /= singleton_op singleton_valid in Hvalid *.
+Qed.
+
+Definition coherent_views SM t1 s1 : Prop :=
+  match s1.(srole), s1.(sdata) with
+  | Init, None => True
+  | Init, Some t2 =>
+    SM !! t2 = Some (SessionData Resp s1.(sinit) s1.(sresp) (Some t1))
+  | Resp, None => False
+  | Resp, Some _ => True
+  end.
+
+Definition session_map_inv SM : iProp :=
+  ∀ t1 s1, ⌜SM !! t1 = Some s1⌝ -∗
+    key_inv s1.(srole) (sowner s1)
+    ∗ key_inv (sroleo s1) (sother s1)
+    ∗ crypto_meta t1 sessionN ()
+    ∗ stermT Sec t1
+    ∗ (if sdata s1 is Some t2 then stermT Sec t2 else True)
+    ∗ ⌜coherent_views SM t1 s1⌝.
+
+Global Instance session_map_inv_persistent SM :
+  Persistent (session_map_inv SM).
+Proof. apply _. Qed.
+
+Lemma session_map_inv_unregistered SM t :
+  crypto_meta_token t (↑sessionN) -∗
+  session_map_inv SM -∗
+  ⌜SM !! t = None⌝.
+Proof.
+iIntros "Hunreg Hinv".
+destruct (SM !! t) as [s_t|] eqn:SM_t=> //.
+iDestruct ("Hinv" $! _ _ SM_t) as "(?&?&Hreg&?)".
+by iDestruct (crypto_meta_meta_token with "Hunreg Hreg") as "[]".
+Qed.
+
+Definition session_inv : iProp :=
+  auth_inv session_name to_session_map session_map_inv.
+
+Definition session_ctx : iProp :=
+  auth_ctx session_name sessionN to_session_map session_map_inv.
+
+Lemma session_alloc lvl kI kR t rl E ot :
+  let kA := if rl is Init then kI else kR in
+  let kB := if rl is Init then kR else kI in
+  let s  := SessionData rl kI kR ot       in
+  ↑sessionN ⊆ E →
+  (if rl is Init then ot = None else is_Some ot) →
+  session_ctx -∗
+  key_inv rl kA -∗
+  crypto_meta_token t (↑sessionN) -∗
+  termT Pub (TKey Enc kB) -∗
+  guarded lvl (key_inv (swap_role rl) kB) -∗
+  stermT lvl t -∗
+  (if ot is Some t' then stermT lvl t' else True) ={E}=∗
+  guarded lvl (session_auth t s ∗ session_frag t s).
+Proof.
+move=> kA kB s sub rl_ot; iIntros "#Hctx #Howner Hunreg #HkB #HkB' #Ht #Ht'".
+case: lvl => //=.
+iMod (auth_empty session_name) as "#Hinit".
+iMod (auth_acc to_session_map session_map_inv
+         with "[Hctx Hinit]") as "Hinv"; try by eauto.
+iDestruct "Hinv" as (SM) "(_ & Hinv & Hclose)".
+iAssert (▷ ⌜SM !! t = None⌝)%I as "# > %Hfresh".
+  iModIntro.
+  by iApply (session_map_inv_unregistered with "[Hunreg] [Hinv]").
+iMod (crypto_meta_set _ () with "Hunreg") as "#Hreg"; eauto.
+rewrite -auth_own_op singleton_op.
+iApply ("Hclose" $! (<[t:=s]>SM)); iSplit.
+  iPureIntro. rewrite /to_session_map fmap_insert.
+  apply alloc_singleton_local_update.
+    by rewrite lookup_fmap Hfresh.
+  by apply session_data_valid.
+iIntros "!>" (t1' s1').
+case: (decide (t = t1')) => [<-|ne].
+  rewrite lookup_insert.
+  iIntros (Hs); case: Hs=> {s1'}<-.
+  do 5![iSplit=> //].
+  rewrite /s; case: (rl) rl_ot=> // rl_ot.
+    by rewrite rl_ot.
+  by case: rl_ot=> t' -> /=.
+rewrite lookup_insert_ne //; iIntros (SM_t1').
+iDestruct ("Hinv" $! _ _ SM_t1') as "(? & ? & ? & ? & ? & %Hcoh)".
+iFrame; iPureIntro.
+move: Hcoh; rewrite /coherent_views.
+case: (srole s1') (sdata s1')=> [|] [t2'|] //.
+case: (decide (t = t2'))=> [<-|?]; first by rewrite Hfresh.
+by rewrite lookup_insert_ne.
+Qed.
+
+Lemma session_alloc_init lvl kA kB tA E :
+  ↑sessionN ⊆ E →
+  session_ctx -∗
+  key_inv Init kA -∗
+  crypto_meta_token tA (↑sessionN) -∗
+  termT Pub (TKey Enc kB) -∗
+  guarded lvl (key_inv Resp kB) -∗
+  stermT lvl tA ={E}=∗
+  guarded lvl (session_auth tA (SessionData Init kA kB None) ∗
+               session_frag tA (SessionData Init kA kB None)).
+Proof.
+iIntros (HE) "#Hctx #HkA Hunreg #HkB #HkB' #HtA".
+by iApply (session_alloc with "Hctx HkA Hunreg HkB HkB' HtA").
+Qed.
+
+Lemma session_alloc_resp lvl kA kB tA tB E :
+  ↑sessionN ⊆ E →
+  session_ctx -∗
+  key_inv Resp kB -∗
+  crypto_meta_token tB (↑sessionN) -∗
+  termT Pub (TKey Enc kA) -∗
+  guarded lvl (key_inv Init kA) -∗
+  stermT lvl tB -∗
+  stermT lvl tA ={E}=∗
+  guarded lvl (session_auth tB (SessionData Resp kA kB (Some tA)) ∗
+               session_frag tB (SessionData Resp kA kB (Some tA))).
+Proof.
+iIntros (?) "#Hctx #HkB Hunreg #HkA #HkA' #HtB #HtA".
+by iApply (session_alloc with "Hctx HkB Hunreg HkA HkA' HtB")=> /=; eauto.
+Qed.
+
+Lemma session_map_auth_included t s SM :
+  {[t := session_data_auth s]} ≼ to_session_map SM ↔
+  SM !! t = Some s.
+Proof.
+split.
+- move=> e; apply/leibniz_equiv.
+  case/singleton_included_l: e=> x [].
+  rewrite lookup_fmap option_equivE.
+  case: (SM !! t)=> [s'|] //= <-.
+  rewrite Some_included; case.
+  + by case=> /= _; rewrite option_equivE.
+  + by rewrite session_data_auth_included=> <-.
+- move=> e; apply/singleton_included_l.
+  exists (session_data_auth_frag s).
+  by rewrite lookup_fmap e /= Some_included session_data_auth_included; eauto.
+Qed.
+
+Lemma session_map_frag_included t s SM :
+  {[t := session_data_frag s]} ≼ to_session_map SM ↔
+  ∃ s', SM !! t = Some s' ∧ to_session_data' s ≼ to_session_data' s'.
+Proof.
+split.
+- case/singleton_included_l=> x [].
+  rewrite lookup_fmap option_equivE.
+  case: (SM !! t)=> [s'|] //= <-.
+  rewrite Some_included; case.
+  + by case=> /=; rewrite option_equivE.
+  + rewrite session_data_frag_included; eauto.
+- case=> s' [H1 H2].
+  apply/singleton_included_l.
+  rewrite lookup_fmap H1 /=.
+  exists (session_data_auth_frag s'); split=> //.
+  by rewrite Some_included session_data_frag_included; right.
+Qed.
+
+Lemma session_key_inv E lvl t s :
+  ↑sessionN ⊆ E →
+  session_ctx -∗
+  guarded lvl (session_frag t s) ={E}=∗
+  ▷ guarded lvl (key_inv s.(srole) (sowner s)).
+Proof.
+move=> sub; iIntros "#Hctx Hterm"; case: lvl => //=.
+iMod (auth_acc to_session_map _ _ _ _ {[t := session_data_frag s]}
+         with "[Hctx Hterm]") as "Hinv"; try by eauto.
+iDestruct "Hinv" as (SM) "(%Hincl & Hinv & Hclose)".
+iAssert (▷ key_inv s.(srole) (sowner s))%I with "[Hinv]" as "#Hs".
+  case/session_map_frag_included: Hincl=> s' [SM_t ss'].
+  iModIntro.
+  rewrite /sowner; case/to_session_data'_included: ss'=> -> [-> [-> _]].
+  by iDestruct ("Hinv" $! _ _ SM_t) as "(?&?&?&?&?&?)".
+by iMod ("Hclose" $! SM {[t := session_data_frag s]} with "[Hinv]"); eauto.
+Qed.
+
+Definition session_inv' t1 s1 : iProp :=
+  key_inv s1.(srole) (sowner s1)
+  ∗ key_inv (sroleo s1) (sother s1)
+  ∗ crypto_meta t1 sessionN ()
+  ∗ stermT Sec t1
+  ∗ (if sdata s1 is Some t2 then stermT Sec t2 else True).
+
+Lemma session_frag_session_inv0 E lvl t s :
+  ↑sessionN ⊆ E →
+  session_ctx -∗
+  guarded lvl (session_frag t s) ={E}=∗
+  ∃ s', ⌜to_session_data' s ≼ to_session_data' s'⌝ ∗
+        ▷ guarded lvl (session_inv' t s').
+Proof.
+move=> sub; iIntros "#Hctx Hterm"; case: lvl => //=.
+  by iExists s.
+iMod (auth_acc to_session_map session_map_inv
+         with "[Hctx Hterm]") as "Hinv"; try by eauto.
+iDestruct "Hinv" as (SM) "(%Hincl & #Hinv & Hclose)".
+case/session_map_frag_included: Hincl=> s' [SM_t ss'].
+iExists s'.
+iAssert (▷ session_inv' t s')%I with "[Hinv]" as "#Hs".
+  iModIntro.
+  iDestruct ("Hinv" $! _ _ SM_t) as "(?&?&?&?&?&?)".
+  by iSplit => //; eauto.
+by iMod ("Hclose" $! SM {[t := session_data_frag s]} with "[Hinv]"); eauto.
+Qed.
+
+Lemma session_frag_session_inv1 E lvl rl kA kB t t' :
+  ↑sessionN ⊆ E →
+  let s := SessionData rl kA kB (Some t') in
+  session_ctx -∗
+  guarded lvl (session_frag t s) ={E}=∗
+  ▷ guarded lvl (session_inv' t s).
+Proof.
+move=> sub s; iIntros "#Hctx #Hterm".
+iMod (session_frag_session_inv0 with "Hctx Hterm") as (s') "[%s_s' Hs']" => //.
+do 2!iModIntro.
+rewrite /session_inv' /sowner /sother /sroleo /=.
+by case/to_session_data'_included: s_s' => <- [] <- [] <- <- /=.
+Qed.
+
+(* TODO: rename *)
+Lemma session_frag_session_inv2 E lvl t s :
+  ↑sessionN ⊆ E →
+  session_ctx -∗
+  termT lvl t -∗
+  guarded lvl (session_frag t s) ={E}=∗
+  ▷ stermT lvl t.
+Proof.
+iIntros (sub) "#Hctx #Ht #Hsess".
+iMod (session_frag_session_inv0 with "Hctx Hsess") as (s') "[%s_s' Hs']" => //.
+iDestruct "Hs'" as "(_&_&_&#Ht'&_)".
+by case: lvl=> //=; do 2!iModIntro; iSplit; eauto.
+Qed.
+
+Lemma session_frag_key_inv E lvl t s :
+  ↑sessionN ⊆ E →
+  session_ctx -∗
+  guarded lvl (session_frag t s) ={E}=∗
+  ▷ guarded lvl (key_inv (srole s) (sowner s)).
+Proof.
+iIntros (sub) "#Hctx #Hsess".
+iMod (session_frag_session_inv0 with "Hctx Hsess") as (s') "[%s_s' Hs']" => //.
+iDestruct "Hs'" as "(#Hk&_)".
+case: lvl=> //=; do 2!iModIntro.
+rewrite /sowner.
+by case/to_session_data'_included: s_s' => [] <- [] <- [] <- _.
+Qed.
+
+Arguments sroleo !_ /.
+Arguments sother !_ /.
+Arguments sowner !_ /.
+
+Lemma session_update lvl kA kB tA tB E :
+  ↑sessionN ⊆ E →
+  session_ctx -∗
+  guarded lvl (session_auth tA (SessionData Init kA kB None)) -∗
+  guarded lvl (session_frag tB (SessionData Resp kA kB (Some tA))) ={E}=∗
+  guarded lvl (session_auth tA (SessionData Init kA kB (Some tB)) ∗
+               session_frag tA (SessionData Init kA kB (Some tB))).
+Proof.
+iIntros (sub) "Hctx HA HB"; case: lvl => //=.
+case: (decide (tA = tB))=> [<-|tAB].
+  iPoseProof (session_agree with "HA HB") as "%agree".
+  by rewrite to_session_data'_included /= in agree *; intuition.
+set s1 := SessionData Init _ _ _; set s2 := SessionData Resp _ _ _.
+pose (f1 := {[tA := session_data_auth s1]} : gmap _ _).
+pose (f2 := {[tB := session_data_frag s2]} : gmap _ _).
+iMod (auth_acc to_session_map _ _ _ _
+         (f1 ⋅ f2) with "[Hctx HA HB]") as "Hinv"; try by eauto.
+  by rewrite auth_own_op; iFrame.
+iDestruct "Hinv" as (SM) "(%Hincl & #Hinv & Hclose)".
+have /session_map_auth_included SM_tA : f1 ≼ to_session_map SM.
+  apply: cmra_included_trans Hincl; exact: cmra_included_l.
+have /session_map_frag_included SM_tB: f2 ≼ to_session_map SM.
+  apply: cmra_included_trans Hincl; exact: cmra_included_r.
+case: SM_tB=> s2' [SM_tB s2_incl].
+move: SM_tB; rewrite -(to_session_data'_included_eq s2_incl) /=; last by eauto.
+move=> SM_tB {s2' s2_incl}.
+set s1' := SessionData Init kA kB (Some tB).
+pose (f1' := {[tA := session_data_auth_frag s1']} : gmap _ _).
+pose (SM' := <[tA := s1']> SM).
+iMod ("Hclose" $! (<[tA := s1']>SM) (f1' ⋅ f2) with "[]") as "Hown"; last first.
+  rewrite /f1' -singleton_op !auth_own_op; iModIntro.
+  by iDestruct "Hown" as "[[??]?]"; iFrame.
+have f2_tA : f2 !! tA = None by rewrite lookup_singleton_ne.
+iSplit.
+  iPureIntro.
+  rewrite /to_session_map fmap_insert -![_ ⋅ f2]insert_singleton_op //.
+  rewrite -(insert_insert f2 tA (session_data_auth_frag s1') (session_data_auth s1)).
+  eapply insert_local_update.
+  - by rewrite lookup_fmap SM_tA.
+  - by rewrite lookup_insert.
+  apply local_update_unital_discrete.
+  intros a _ <-%cancelable=> //; last by apply _.
+  split=> //; first exact: session_data_auth_frag_valid.
+  rewrite {2}/session_data_auth_frag -cmra_assoc -auth_frag_op -Some_op.
+  by rewrite /to_session_data' /= -!pair_op !agree_idemp.
+iIntros "!>" (t s).
+case: (decide (tA = t))=> [<-|ne].
+  rewrite lookup_insert; iIntros (e); case: e=> ?; subst s.
+  iDestruct ("Hinv" $! _ _ SM_tA) as "(?&?&?&?&?&?)".
+  iDestruct ("Hinv" $! _ _ SM_tB) as "(?&?&?&?&?&?)".
+  do 5![iSplit=> //]; iPureIntro.
+  rewrite /s1' /=.
+  by rewrite /coherent_views /= lookup_insert_ne // SM_tB.
+rewrite lookup_insert_ne //.
+iIntros "%SM_t"; iDestruct ("Hinv" $! _ _ SM_t) as "(?&?&?&?&?&%Hcoh)".
+do 5![iSplit=> //]; iPureIntro.
+move: Hcoh; rewrite /coherent_views.
+case erole: (srole s)=> //.
+case edata: (sdata s)=> [t'|] //.
+case: (decide (tA = t'))=> [<-|?]; first by rewrite SM_tA.
+by rewrite lookup_insert_ne.
+Qed.
+
+End Session.
